\question Q1\droppoints

\begin{solution}
    From the definition of probability distribution and expectation, we have

    \[
        \sum_{x}{p(x)} = 1 \quad \text{and} \quad \mathbb{E}[f] = \sum_{x}{p(x)f(x)}
    \]

    To express the variance, we expand the square:

    \[
        \mathbb{V}[f]
        = \mathbb{E}[(f - \mathbb{E}[f])^2]
        = \mathbb{E}[f^2 - 2f \cdot \mathbb{E}[f] + (\mathbb{E}[f])^2)]
    \]

    Rewriting the expectation using summation notation:

    \[
        \mathbb{V}[f]
        = \sum_{x}{pf^2} - \sum_{x}{2pf\mathbb{E}[f]} + \sum_{x}{pE[f]^2}
    \]

    Since $\mathbb{E}[f]$ is a constant (the mean of the probability density function $f(x)$), we can factor it out of the summation:

    \begin{align*}
        \mathbb{V}[f]
        &= \sum_{x}{pf^2} - 2\mathbb{E}[f]\sum_{x}{pf} + E[f]^2\sum_{x}{p} \\
        &= \sum_{x}{pf^2} - 2\mathbb{E}[f] \cdot \mathbb{E}[f] \cdot + E[f]^2 \cdot 1 \\
        &= \sum_{x}{pf^2} - E[f]^2
    \end{align*}

    Rewriting $\sum_{x}{pf^2}$ as $\mathbb{E}[\cdot]$, we arrive at final form:

    \[
        \mathbb{V}[f] = \mathbb{E}[f^2] - E[f]^2
    \]

    In the case of continuous variables, a similar approach can be used to deduce the formula for variance.
\end{solution}
