\question Q1\droppoints

\begin{solution}
    \text{(a)} \textbf{Proof.} By the definition of $\tanh$, we have

    \[
        \begin{align*}
            \tanh(a)
            &= \frac{e^x - e^{-x}}{e^x + e^{-x}} & \\
            &= \frac{1 - e^{-2x}}{1 + e^{-2x}} & \text{(Cancel out } ${e^x}$ \text{)} \\
            &= \frac{2 - (1 + e^{-2a})}{1 + e^{-2x}} & \\
            &= 2 \cdot \frac{1}{1 + e^{-2x}} - 1 & \\
            &= 2\sigma(2a) - 1
        \end{align*}
    \]

    \text{(b)} \textbf{Proof.} Let us denote
    \[
        z(x, \mathbf{u}) = u_0 + \sum_{j=1}^{M}{u_j \sigma \left(\frac{x - \mu_j}{s}\right)}.
    \]

    From the conclusion of part (a), we have:
    \begin{align*}
        y(x, \mathbf{u})
        &= u_0 + \sum_{j=1}^{M}{u_j \tanh \left(\frac{x - \mu_j}{2s}\right)} \\[0.5em]
        &= u_0 + \sum_{j=1}^{M}{u_j \left[ 2\sigma \left(\frac{x - \mu_j}{s}\right) - 1 \right]} \\[0.5em]
        &= u_0 + \sum_{j=1}^{M}{2u_j\sigma\left(\frac{x - \mu_j}{s}\right)} - \sum_{j=1}^{M}{u_j} \\[0.5em]
        &= \left(u_0 - \sum_{j=1}^{M}{u_j}\right) + \sum_{j=1}^{M}{2u_j\sigma\left(\frac{x - \mu_j}{s}\right)} \\[0.5em]
        &= z(x, \mathbf{w})
    \end{align*}

    \text{(c)} The relationship between $\mathbf{u}$ and $\mathbf{w}$ in part \text{(b)} is as follows:

    \[
        w_0 = u_0 - \sum_{j=1}^{M}{u_j}
    \]

    and $w_j = 2u_j$ for $1 \leq j \leq M$.

\end{solution}